theories/Distr.ec
@@ -13,18 +13,34 @@ require import Fun.
 
 op charfun (p:'a -> bool) x: real = if p x then 1%r else 0%r.
 
-op mu_x (d:'a distr) x: real = mu d ((=) x).
+op mu_x (d:'a distr) x: real = mu d (pred1 x).
 
-op weight (d:'a distr): real = mu d True.
+op weight (d:'a distr): real = mu d predT.
 
 op in_supp x (d:'a distr) : bool = 0%r < mu_x d x.
 
 op support (d:'a distr) x = in_supp x d.
 
-pred isuniform (d:'a distr) = forall (x y:'a),
-  in_supp x d =>
-  in_supp y d =>
-  mu_x d x = mu_x d y.
+pred is_lossless (d : 'a distr) = mu d predT = 1%r.
+
+pred is_full (d : 'a distr) = forall x, support d x.
+
+pred is_subuniform (d : 'a distr) = forall (x y:'a),
+  support d x =>
+  support d y =>
+  mu d (pred1 x) = mu d (pred1 y).
+
+pred is_uniform (d : 'a distr) =
+     is_lossless d
+  /\ is_subuniform d.
+
+pred is_subuniform_over (d : 'a distr) (p : 'a -> bool) =
+     (forall x, support d x <=> p x)
+  /\ is_subuniform d.
+
+pred is_uniform_over (d : 'a distr) (p : 'a -> bool) =
+     (forall x, support d x <=> p x)
+  /\ is_uniform d.
 
 (** Point-wise equality *)
 pred (==)(d d':'a distr) =
@@ -38,26 +54,25 @@ pred (===)(d d':'a distr) =
 axiom mu_bounded (d:'a distr) (p:'a -> bool):
   0%r <= mu d p <= 1%r.
 
-axiom mu_false (d:'a distr): mu d False = 0%r.
+axiom mu_false (d:'a distr): mu d pred0 = 0%r.
 
 axiom mu_sub (d:'a distr) (p q:('a -> bool)):
   p <= q => mu d p <= mu d q.
 
 axiom mu_supp_in (d:'a distr) p:
-  mu d p = mu d True <=>
+  mu d p = mu d predT <=>
   support d <= p.
 
 axiom mu_or (d:'a distr) (p q:('a -> bool)):
-  mu d (p \/ q) = mu d p + mu d q - mu d (p /\ q).
+  mu d (predU p q) = mu d p + mu d q - mu d (predI p q).
 
 axiom pw_eq (d d':'a distr):
   d == d' <=> d = d'.
 
 axiom uniform_unique (d d':'a distr):
-  mu d True = mu d' True =>
   support d = support d' =>
-  isuniform d  =>
-  isuniform d' =>
+  is_uniform d  =>
+  is_uniform d' =>
   d = d'.
 
 (** Lemmas *)
@@ -73,107 +88,104 @@ qed.
 
 lemma ew_eq (d d':'a distr):
   d === d' => d = d'.
-proof strict.
+proof.
 intros=> ew_eq; rewrite -pw_eq=> x.
 by rewrite /mu_x ew_eq.
 qed.
 
 lemma nosmt mu_or_le (d:'a distr) (p q:'a -> bool) r1 r2:
   mu d p <= r1 => mu d q <= r2 =>
-  mu d (p \/ q) <= r1 + r2 by [].
+  mu d (predU p q) <= r1 + r2 by [].
 
 lemma nosmt mu_and  (d:'a distr) (p q:'a -> bool):
-  mu d (p /\ q) = mu d p + mu d q - mu d (p \/ q)
+  mu d (predI p q) = mu d p + mu d q - mu d (predU p q)
 by [].
 
 lemma nosmt mu_and_le_l (d:'a distr) (p q:'a -> bool) r:
   mu d p <= r =>
-  mu d (p /\ q) <= r.
-proof strict.
+  mu d (predI p q) <= r.
+proof.
 apply (Real.Trans _ (mu d p)).
-by apply mu_sub; rewrite /Pred.(/\)=> x.
+by apply mu_sub; rewrite /predI=> x.
 qed.
 
 lemma nosmt mu_and_le_r (d:'a distr) (p q:'a -> bool) r :
   mu d q <= r => 
-  mu d (p /\ q) <= r.
-proof strict.
+  mu d (predI p q) <= r.
+proof.
 apply (Real.Trans _ (mu d q)).
-by apply mu_sub; rewrite /Pred.(/\)=> x.
+by apply mu_sub; rewrite /predI=> x.
 qed.
 
 lemma mu_supp (d:'a distr):
-  mu d (support d) = mu d True.
-proof strict.
-by rewrite mu_supp_in.
-qed.
+  mu d (support d) = mu d predT.
+proof. by rewrite mu_supp_in. qed.
 
 lemma mu_eq (d:'a distr) (p q:'a -> bool):
   p == q => mu d p = mu d q.
-proof strict.
+proof.
 by intros=> ext_p_q; congr=> //; apply fun_ext.
 qed.
 
 lemma mu_disjoint (d:'a distr) (p q:('a -> bool)):
-  (p /\ q) <= False =>
-  mu d (p \/ q) = mu d p + mu d q.
-proof strict.
+  (predI p q) <= pred0 =>
+  mu d (predU p q) = mu d p + mu d q.
+proof.
 intros=> and_p_q_false; rewrite mu_or.
-cut ->: (p /\ q) = False by apply leq_asym.
+cut ->: (predI p q) = pred0 by apply subpred_asym.
 by rewrite mu_false.
 qed.
 
 lemma mu_not (d:'a distr) (p:('a -> bool)):
-  mu d (!p) = mu d True - mu d p.
-proof strict.
-cut ->: forall (x y z:real), x = y - z <=> x + z = y by smt.
-rewrite -mu_disjoint 2:Excluded_Middle //.
-by apply leq_refl; apply Sound.
+  mu d (predC p) = mu d predT - mu d p.
+proof.
+have: mu d (predC p) + mu d p = mu d predT; [rewrite -mu_disjoint | smt].
++ by rewrite predCpredI; apply/(subpred_refl<:'a> pred0). (* rewrite seems to unroll too much *)
++ by rewrite predCpredU.
 qed.
 
 lemma mu_split (d:'a distr) (p q:('a -> bool)):
-  mu d p = mu d (p /\ q) + mu d (p /\ !q).
-proof strict.
+  mu d p = mu d (predI p q) + mu d (predI p (predC q)).
+proof.
 rewrite -mu_disjoint; first smt.
-by apply mu_eq; smt.
+by apply mu_eq=> x; rewrite /predI /predC /predU !(andC (p x)) orDandN.
 qed.
 
 lemma mu_support (p:('a -> bool)) (d:'a distr):
-  mu d p = mu d (p /\ (support d)).
-proof strict.
-apply Antisymm; last by apply mu_sub; apply And_leq_l.
-cut ->: forall (p q:'a -> bool), (p /\ q) = !((!p) \/ (!q))
-  by (intros=> p' q'; apply fun_ext; smt).
+  mu d p = mu d (predI p (support d)).
+proof.
+apply Antisymm; last by apply/mu_sub/predIsubpredl.
+have ->: forall (p q:'a -> bool), (predI p q) = predC (predU (predC p) (predC q)).
+  by (move=> p1 p2; apply fun_ext; delta; smt). (* delta *)
 by rewrite mu_not mu_or !mu_not mu_supp; smt.
 qed.
 
 lemma witness_support P (d:'a distr):
   0%r < mu d P <=> (exists x, P x /\ in_supp x d).
 proof.
-split.
+split=> [|[] x [x_in_P x_in_d]].
   rewrite mu_support=> nzero.
   apply witness_nzero in nzero; case nzero=> x.
-  rewrite /Pred.(/\) /support //= => p_supp.
+  rewrite /predI //= => p_supp.
   by exists x.
-  move=> [] x [x_in_P x_in_d].
-  cut: mu d ((=) x) <= mu d P /\ 0%r < mu d ((=) x); last smt.
-  split; last by rewrite x_in_d.
-  by rewrite mu_sub // /Pred.(<=)=> x0 <<-.
+cut: mu d (pred1 x) <= mu d P /\ 0%r < mu d (pred1 x); last smt.
+split=> [|//=].
+by rewrite mu_sub // /Pred.(<=) /pred1 => x0 <<-.
 qed.
 
 lemma mu_sub_support (d:'a distr) (p q:('a -> bool)):
-  (p /\ (support d)) <= (q /\ (support d)) =>
+  (predI p (support d)) <= (predI q (support d)) =>
   mu d p <= mu d q.
-proof strict.
-by intros=> ple_p_q; rewrite (mu_support p) (mu_support q);
+proof.
+by move=> ple_p_q; rewrite (mu_support p) (mu_support q);
    apply mu_sub.
 qed.
 
 lemma mu_eq_support (d:'a distr) (p q:('a -> bool)):
-  (p /\ (support d)) = (q /\ (support d)) =>
+  (predI p (support d)) = (predI q (support d)) =>
   mu d p = mu d q.
-proof strict.
-by intros=> eq_supp;
+proof.
+by move=> eq_supp;
    rewrite (mu_support p) (mu_support q);
    apply mu_eq; rewrite eq_supp.
 qed.
@@ -183,10 +195,10 @@ lemma weight_0_mu (d:'a distr):
 by [].
 
 lemma mu_one (P:'a -> bool) (d:'a distr):
-  P == True => 
+  P == predT => 
   weight d = 1%r =>
   mu d P = 1%r.
-proof strict.
+proof.
 intros=> heq <-.
 rewrite /weight.
 congr=> //.
@@ -202,13 +214,12 @@ theory Dempty.
 
   lemma unique (d:'a distr):
     weight d = 0%r <=> d = dempty.
-  proof strict.
+  proof.
   split; last smt.
   by intros weight_0; rewrite -(pw_eq<:'a> d dempty); smt.
   qed.
 
-  lemma demptyU: isuniform dempty<:'a>. admit. qed.
-
+  lemma demptyU: is_subuniform dempty<:'a> by smt.
 end Dempty.
 
 (** Point distribution *)
@@ -228,7 +239,7 @@ theory Dunit.
 
   lemma nosmt mu_x_def (x y:'a):
     mu_x (dunit y) x = if x = y then 1%r else 0%r
-  by rewrite /mu_x mu_def /charfun.
+  by rewrite /mu_x mu_def /charfun pred1E.
 
   lemma nosmt mu_x_def_eq (x:'a):
     mu_x (dunit x) x = 1%r
@@ -247,7 +258,7 @@ theory Dunit.
   by [].
 
   lemma dunitU (x:'a):
-    isuniform (dunit x)
+    is_uniform (dunit x)
   by [].
 end Dunit.
 
@@ -284,14 +295,17 @@ theory Dinter.
     i <= j => 
     mu (dinter i j) (fun x, i <= x <= j) = 1%r.
   proof strict.
-    move=> h; rewrite -(mu_eq_support (dinter i j) True).
+    move=> h; rewrite -(mu_eq_support (dinter i j) predT).
       by apply/fun_ext=> x /=; smt.
       by smt.
   qed.
 
   lemma dinterU (i j:int):
-    isuniform (dinter i j)
-  by [].
+    is_subuniform (dinter i j).
+  proof.
+    move=> x y x_in_supp y_in_supp.
+    by rewrite -/(mu_x _ x) -/(mu_x _ y) !mu_x_def_in.
+  qed.
 end Dinter.
 
 (** Normalization of a sub-distribution *)
@@ -320,7 +334,7 @@ theory Dscale.
   qed.  
 
   lemma dscaleU (d:'a distr):
-    isuniform d => isuniform (dscale d)
+    mu d predT <> 0%r => is_subuniform d => is_uniform (dscale d)
   by [].
 end Dscale.
 
@@ -329,28 +343,27 @@ theory Dapply.
   op dapply: ('a -> 'b) -> 'a distr -> 'b distr.
 
   axiom mu_def (d:'a distr) (f:'a -> 'b) P:
-    mu (dapply f d) P = mu d (fun x, P (f x)).
+    mu (dapply f d) P = mu d (preim f P).
 
   lemma mu_x_def (d:'a distr) (f:'a -> 'b) x:
-    mu_x (dapply f d) x = mu d (fun y, x = f y).
-  proof strict.
-  by rewrite /mu_x mu_def.
-  qed.
+    mu_x (dapply f d) x = mu d (preim f (pred1 x)).
+  proof. by rewrite /mu_x mu_def. qed.
 
   lemma supp_def (d:'a distr) (f:'a -> 'b) y:
     in_supp y (dapply f d) <=> exists x, y = f x /\ in_supp x d.
-  proof strict.
+  proof.
   rewrite /in_supp /mu_x mu_def; split.
-    rewrite mu_support /Pred.(/\) /= => in_sup. smt.
+    rewrite mu_support /predI /= => in_sup. smt.
     intros=> [x]; rewrite /in_supp /mu_x=> [y_def nempty].
-    cut : (=) x <= (fun x, y = f x) by (by intros=> w).
+    have: pred1 x <= preim f (pred1 y)
+      by move=> w; rewrite !pred1E. 
     smt.
   qed.
 
   lemma lossless (d : 'a distr) (f : 'a -> 'b):
     weight (dapply f d) = weight d.
-  proof strict.
-  by rewrite /weight mu_def /True.
+  proof.
+  by rewrite /weight mu_def.
   qed.
 
   lemma dapply_preim (d:'a distr) (f:'a -> 'b) P:
@@ -366,41 +379,14 @@ theory Dapply.
     (forall x, P x => g (f x) = x) =>
     (forall y, f (g y) = y) =>
     support d <= P =>
-    mu (dapply f d) ((=) x) = mu d ((=) (g x)).
+    mu (dapply f d) (pred1 x) = mu d (pred1 (g x)).
   proof.
     move=> fK gK leq_supp_P.
-    rewrite mu_def /= (mu_support (fun y, x = f y)) (mu_support ((=) (g x))); apply mu_eq=> x0.
-    rewrite /Pred.(/\) eq_iff /=; split.
-      by case => f_x0 sup_x0; split=> //; rewrite -fK 1:leq_supp_P // -f_x0.
-      by case => x0_g supp_x0; split=> //; rewrite -(gK x) x0_g.
+    rewrite mu_def /= (mu_support (preim f (pred1 x))) (mu_support (pred1 (g x))); apply mu_eq=> x0.
+    rewrite /predI eq_iff /=; split.
+      by case => f_x0 sup_x0; split=> //; rewrite -fK 1:leq_supp_P//;
+         move: f_x0; rewrite /preim /pred1. (* Why? *)
+      by case => x0_g sup_x0; split=> //; rewrite -(gK x) /preim /pred1;
+         move: x0_g; rewrite /pred1. (* Why? *)
   qed.
 end Dapply.
-
-(** Laplacian *) (* TODO: This is drafty! *)
-theory Dlap.
-  op dlap : int -> real -> int distr.
-
-  axiom in_supp mean scale x:
-    0%r <= scale => in_supp x (dlap mean scale).
-
-(*
-  axiom mu_x_def : forall (mean:int, scale:real, x:int),
-    0%r <= scale => 
-    mu_x (dlap mean scale) x = 
-      (1%r / (2%r*scale))
-    * real.exp( - (| x%r - mean%r|)) / scale. 
-*)
-
-  axiom lossless mean scale:
-    0%r <= scale => weight (dlap mean scale) = 1%r.
-(* x = $dlap(x1,s)   ~ x = $dlap(0,s) + x1 : ={x1,s} ==> ={x}. *)
-end Dlap.
-
-(* ---------------------------------------------------------------------- *)
-
-(* intergral of f in a distribution d *)
-op muf : ('a -> real) -> 'a distr -> real.
-
-(* Injection of bool into real *) 
-op b2r (b:bool) = if b then 1%r else 0%r.
-
