theories/newth/StdBigop.ec
@@ -5,39 +5,51 @@
  * Distributed under the terms of the CeCILL-B-V1 license
  * -------------------------------------------------------------------- *)
 
-require NewBigop.
-
+(* -------------------------------------------------------------------- *)
+require import Pred Int IntExtra Real Ring List.
+require (*--*) NewBigop NewBigalg.
 
 (* -------------------------------------------------------------------- *)
-require import Int.
-
-clone NewBigop as BIA with
+theory BIA.
+clone include NewBigalg with
   type t <- int,
-  op Support.idm <- 0,
-  op Support.(+)  <- Int.( + )
-  proof Support.Axioms.* by (delta;smt).
+  op ZM.zeror <- 0,
+  op ZM.( + ) <- Int.(+),
+  op ZM.( - ) <- Int.(-),
+  op ZM.([-]) <- Int.([-])
+  proof ZM.* by smt.
+
+  lemma nosmt sumzE ss : sumz ss = BIA.big predT (fun x => x) ss.
+  proof. by elim: ss=> [|s ss ih] //=; rewrite BIA.big_cons -ih. qed.
+      
+  lemma nosmt big_constz (P : 'a -> bool) x s:
+    big P (fun i => x) s = x * (count P s).
+  proof.
+    rewrite big_const -Support.iteropE -IntID.intmulpE.
+    by apply/count_ge0. by rewrite IntID.intmulz mulzC.
+  qed.  
+end BIA.
 
 clone NewBigop as BIM with
   type t <- int,
   op Support.idm <- 1,
-  op Support.(+)  <- Int.( * )
-  proof Support.Axioms.* by (delta;smt).
-
+  op Support.(+) <- Int.( * )
+  proof Support.Axioms.* by smt.
 
 (* -------------------------------------------------------------------- *)
-require import Real.
-
-clone NewBigop as BRA with
+clone NewBigalg as BRA with
   type t <- real,
-  op Support.idm <- 0%r,
-  op Support.(+)  <- Real.( + )
-  proof Support.Axioms.* by (delta;smt).
+  op ZM.zeror <- 0%r,
+  op ZM.( + ) <- Real.(+),
+  op ZM.( - ) <- Real.(-),
+  op ZM.([-]) <- Real.([-])
+  proof ZM.* by smt.
 
 clone NewBigop as BRM with
   type t <- real,
   op Support.idm <- 1%r,
-  op Support.(+)  <- Real.( * )
-  proof Support.Axioms.* by (delta;smt).
+  op Support.(+) <- Real.( * )
+  proof Support.Axioms.* by smt.
 
 (* -------------------------------------------------------------------- *)
 require import Bool.
@@ -45,8 +57,8 @@ require import Bool.
 clone NewBigop as BBA with
   type t <- bool,
   op Support.idm <- false,
-  op Support.(+)  <- Bool.( ^^ )
-  proof Support.Axioms.* by (delta;smt).  
+  op Support.(+) <- Bool.( ^^ )
+  proof Support.Axioms.* by (delta; smt).  
 
 clone NewBigop as BBM with
   type t <- bool,
