theories/crypto/Birthday.ec
@@ -1,0 +1,274 @@
+(* --------------------------------------------------------------------
+ * Copyright (c) - 2012--2015 - IMDEA Software Institute
+ * Copyright (c) - 2012--2015 - Inria
+ * 
+ * Distributed under the terms of the CeCILL-B-V1 license
+ * -------------------------------------------------------------------- *)
+
+require import Option.
+require import Int.
+require import Real.
+require import Distr.
+require import List.
+require (*--*) Sum.
+(*---*) import Monoid.
+require (*--*) Mu_mem.
+
+(** A non-negative integer q **)
+op q:int.
+axiom lt0q: 0 < q.
+
+(** A type T equipped with its full uniform distribution **)
+type T.
+
+op uT: T distr.
+axiom uT_ufT: is_uniform_over uT predT.
+
+(** A module that samples in uT on queries to s **)
+module Sample = {
+  var l:T list
+
+  proc init(): unit = {
+    l = [];
+  }
+
+  proc s(): T = {
+    var r;
+
+    r = $uT;
+    l = r::l;
+    return r;
+  }
+}.
+
+module type Sampler = {
+  proc init(): unit
+  proc s(): T
+}.
+
+(** Adversaries that may query an s oracle **)
+module type ASampler = {
+  proc s(): T
+}.
+
+module type Adv(S:ASampler) = {
+  proc a(): unit
+}.
+
+(** And an experiment that initializes the sampler and runs the adversary **)
+module Exp(S:Sampler,A:Adv) = {
+  module A = A(S)
+
+  proc main(): unit = {
+    S.init();
+    A.a();
+  }
+}.
+
+(** Forall adversary A that makes at most q queries to its s oracle,
+    the probability that the same output is sampled twice is bounded
+    by q^2/|T|                                                        **)
+section.
+  declare module A:Adv {Sample}.
+  axiom A_ll (S <: ASampler {A}): islossless S.s => islossless A(S).a.
+  axiom A_bounded &m: size Sample.l{m} = 0 => Pr[A(Sample).a() @ &m: size Sample.l <= q] = 1%r.
+
+  local hoare hl_A_bounded: A(Sample).a: size Sample.l = 0 ==> size Sample.l <= q.
+  proof.
+    hoare.
+    phoare split ! 1%r 1%r=> //=.
+      conseq (A_ll Sample _).
+        by proc; auto=> //=; rewrite -/predT; smt. (* FIXME: -delta *)
+    by bypr=> &m l_empty; rewrite (A_bounded &m l_empty).
+  qed.
+
+  local module BSample = {
+    proc init = Sample.init
+
+    proc s(): T = {
+      var r = witness;
+
+      if (size Sample.l < q) {
+        r = $uT;
+        Sample.l = r::Sample.l;
+      }
+      return r;
+    }
+  }.
+
+  local equiv eq_Sample_BSample: Exp(Sample,A).main ~ Exp(BSample,A).main: ={glob A} ==> ={Sample.l}.
+  proof.
+    symmetry.
+    proc.
+    conseq (_: ={glob A} ==> size Sample.l{2} <= q => ={Sample.l}) _ (_: true ==> size Sample.l <= q); first 2 smt.
+      call hl_A_bounded.
+      by inline*; auto; smt.
+    call (_: !size Sample.l <= q, ={Sample.l})=> //=.
+      exact A_ll.
+      by proc; sp; if{1}=> //=; auto; smt.
+      by move=> &2 bad; proc; sp; if=> //=; auto; rewrite -/predT; smt. (* FIXME: -delta *)
+      by proc; auto; rewrite -/predT; smt. (* FIXME: -delta *)
+    by inline *; auto; smt.
+  qed.
+
+  local lemma pr_BSample &m:
+    Pr[Exp(BSample,A).main() @ &m: size Sample.l <= q /\ !uniq Sample.l]
+    <= (q^2)%r * mu uT (pred1 witness).
+  proof.
+    fel 1 (size Sample.l) (fun x, q%r * mu uT (pred1 witness)) q (!uniq Sample.l) [BSample.s: (size Sample.l < q)]=> //.
+     rewrite Sum.int_sum_const //= Sum.intval_card_0 1:smt /=.
+      cut ->: q^2 = q * q; last by smt.
+      rewrite (_: 2 = 1 + 1) // -Int.pow_add //.
+      by rewrite (_: q^1 = q) // (_: 1 = 0 + 1) 1:// powS // pow0.
+      by inline*; auto; smt.
+      proc; sp; if=> //; last by (hoare; auto; smt).
+      wp; rnd (mem Sample.l); skip=> //=.
+      progress.
+        have:= Mu_mem.mu_mem_le_size (Sample.l{hr}) uT (mu uT (pred1 witness)) _.
+          move=> x _; rewrite /mu_x; cut: mu uT (pred1 x) = mu uT (pred1 witness); last smt.
+          have [uT_fu [_ uT_suf]]:= uT_ufT.
+          by apply uT_suf; apply uT_fu.
+        move /(Trans _ ((size Sample.l{hr})%r * mu uT (pred1 witness)))=> -> //=.
+        by apply/mulrMle; smt.
+        by move: H4; rewrite H0.
+      by progress; proc; rcondt 2; auto; smt.
+      by progress; proc; rcondf 2; auto.
+  qed.
+
+  lemma pr_collision &m:
+    Pr[Exp(Sample,A).main() @ &m: !uniq Sample.l]
+    <= (q^2)%r * mu uT (pred1 witness).
+  proof.
+    cut ->: Pr[Exp(Sample,A).main() @ &m: !uniq Sample.l]
+            = Pr[Exp(BSample,A).main() @ &m: size Sample.l <= q /\ !uniq Sample.l].
+      byequiv (_: ={glob A} ==> ={Sample.l} /\ size Sample.l{2} <= q)=> //=.
+      conseq eq_Sample_BSample _ (_: _ ==> size Sample.l <= q)=> //=.
+        proc.
+        call (_: size Sample.l <= q).
+          by proc; sp; if=> //=; auto; smt.
+        by inline *; auto; smt.
+    by apply (pr_BSample &m).
+  qed.
+end section.
+
+(*** The same result using a bounding module ***)
+(** TODO: factor out the second step of the proof (pr_BSample)
+    and exercise some modularity **)
+module Bounder(S:Sampler) = {
+  var c:int
+
+  proc init(): unit = {
+    S.init();
+    c = 0;
+  }
+
+  proc s(): T = {
+    var r = witness;
+
+    if (c < q) {
+      r = S.s();
+      c = c + 1;
+    }
+    return r;
+  }
+}.
+
+module ABounder(S:ASampler) = {
+  proc s(): T = {
+    var r = witness;
+
+    if (Bounder.c < q) {
+      r = S.s();
+      Bounder.c = Bounder.c + 1;
+    }
+    return r;
+  }
+}.
+
+module Bounded(A:Adv,S:ASampler) = {
+  proc a(): unit = {
+    Bounder.c = 0;
+    A(ABounder(S)).a();
+  }
+}.
+
+equiv PushBound (S <: Sampler {Bounder}) (A <: Adv {S,Bounder}):
+  Exp(Bounder(S),A).main ~ Exp(S,Bounded(A)).main:
+    ={glob A,glob S} ==>
+    ={glob A,glob S}.
+proof. by proc; inline*; sim. qed.
+
+(** Forall adversary A with access to the bounded s oracle, the
+    probability that the same output is sampled twice is bounded by
+    q^2/|T|                                                         **)
+section.
+  declare module A:Adv {Sample,Bounder}.
+
+  axiom A_ll (S <: ASampler {A}): islossless S.s => islossless A(S).a.
+
+  local module BSample = {
+    proc init = Sample.init
+
+    proc s(): T = {
+      var r = witness;
+
+      if (size Sample.l < q) {
+        r = $uT;
+        Sample.l = r::Sample.l;
+      }
+      return r;
+    }
+  }.
+
+  local equiv eq_Sample_BSample: Exp(Bounder(Sample),A).main ~ Exp(BSample,A).main: ={glob A} ==> ={Sample.l}.
+  proof.
+    transitivity  Exp(Sample,Bounded(A)).main 
+                  (={glob A,glob Sample} ==> ={glob A,glob Sample})
+                  (={glob A} ==> ={Sample.l})=> //.
+    + by progress; exists (glob A){2}, Sample.l{1}.
+    + exact (PushBound Sample A).
+    proc; inline*.
+    call (_: ={glob Sample} /\ Bounder.c{1} = size Sample.l{1}).
+      by proc; sp; if=> //; inline Sample.s; auto; smt.
+    by auto.
+  qed.
+
+  local lemma pr_BSample &m:
+    Pr[Exp(BSample,A).main() @ &m: size Sample.l <= q /\ !uniq Sample.l]
+    <= (q^2)%r * mu uT (pred1 witness).
+  proof.
+    fel 1 (size Sample.l) (fun x, q%r * mu uT (pred1 witness)) q (!uniq Sample.l) [BSample.s: (size Sample.l < q)]=> //.
+      rewrite Sum.int_sum_const //= Sum.intval_card_0 1:smt /=.
+      cut ->: q^2 = q * q; last by smt.
+      rewrite (_: 2 = 1 + 1) // -Int.pow_add //.
+      by rewrite (_: q^1 = q) // (_: 1 = 0 + 1) 1:// powS // pow0.
+      by inline*; auto; smt.
+      proc; sp; if=> //; last by (hoare; auto; smt).
+      wp; rnd (mem Sample.l); skip=> //=.
+      progress.
+        have:= Mu_mem.mu_mem_le_size (Sample.l{hr}) uT (mu uT (pred1 witness)) _.
+          move=> x _; rewrite /mu_x; cut: mu uT (pred1 x) = mu uT (pred1 witness); last smt.
+          have [uT_fu [_ uT_suf]]:= uT_ufT.
+          by apply uT_suf; apply uT_fu.
+        move /(Trans _ ((size Sample.l{hr})%r * mu uT (pred1 witness)))=> -> //=.
+        by apply/mulrMle; smt.
+        by move: H4; rewrite H0.
+      by progress; proc; rcondt 2; auto; smt.
+      by progress; proc; rcondf 2; auto.
+  qed.
+
+  lemma pr_collision_bounded_oracles &m:
+    Pr[Exp(Bounder(Sample),A).main() @ &m: !uniq Sample.l]
+    <= (q^2)%r * mu uT (pred1 witness).
+  proof.
+    cut ->: Pr[Exp(Bounder(Sample),A).main() @ &m: !uniq Sample.l]
+            = Pr[Exp(BSample,A).main() @ &m: size Sample.l <= q /\ !uniq Sample.l].
+      byequiv (_: ={glob A} ==> ={Sample.l} /\ size Sample.l{2} <= q)=> //=.
+      conseq eq_Sample_BSample _ (_: _ ==> size Sample.l <= q)=> //=.
+        proc.
+        call (_: size Sample.l <= q).
+          by proc; sp; if=> //=; auto; smt.
+        by inline *; auto; smt.
+    by apply (pr_BSample &m).
+  qed.
+end section.
