theories/crypto/DiffieHellman.ec
@@ -1,0 +1,165 @@
+(* --------------------------------------------------------------------
+ * Copyright (c) - 2012--2015 - IMDEA Software Institute
+ * Copyright (c) - 2012--2015 - Inria
+ * 
+ * Distributed under the terms of the CeCILL-B-V1 license
+ * -------------------------------------------------------------------- *)
+
+require import FSet Int Real.
+require (*  *) Duni.
+require (*  *) CyclicGroup.
+
+clone export CyclicGroup as G.
+
+theory DDH.
+   
+  module type Adversary = {
+    proc guess(gx gy gz:G.group): bool
+  }.
+
+  module DDH0 (A:Adversary) = {
+    proc main() : bool = {
+      var b, x, y;
+      x = $FDistr.dt;
+      y = $FDistr.dt;
+      b = A.guess(g ^ x, g ^ y, g ^ (x*y));
+      return b;
+    }
+  }.
+
+  module DDH1 (A:Adversary) = {
+    proc main() : bool = {
+      var b, x, y, z;
+        
+      x = $FDistr.dt;
+      y = $FDistr.dt;
+      z = $FDistr.dt;
+      b = A.guess(g ^ x, g ^ y, g ^ z);
+      return b;
+    }
+  }.
+
+end DDH.
+  
+
+
+(** Computational Diffie-Hellman problem **)
+theory CDH.
+
+  module type Adversary = {
+    proc solve(gx gy:group): group
+  }.
+
+  module CDH (A:Adversary) = {
+    proc main(): bool = {
+      var x, y, r;
+
+      x = $FDistr.dt;
+      y = $FDistr.dt;
+      r = A.solve(g ^ x, g ^ y);
+      return (r = g ^ (x * y));
+    }
+  }.
+end CDH.
+
+(** Set version of the Computational Diffie-Hellman problem **)
+theory Set_CDH.
+
+  const n: int.
+
+  module type Adversary = {
+    proc solve(gx:group, gy:group): group fset
+  }.
+
+  module SCDH (B:Adversary) = {
+    proc main(): bool = {
+      var x, y, s;
+
+      x = $FDistr.dt;
+      y = $FDistr.dt;
+      s = B.solve(g ^ x, g ^ y);
+      return (mem s (g ^ (x * y)) /\ card s <= n);
+    }
+  }.
+
+  module CDH_from_SCDH (A:Adversary): CDH.Adversary = {
+    proc solve(gx:group, gy:group): group = {
+      var s, x;
+
+      s = A.solve(gx, gy);
+      x = $Duni.dU s;
+      return x;
+    }
+  }.
+
+  (** Naive reduction to CDH **)
+  section.
+    declare module A: Adversary.
+
+    local module SCDH' = {
+      var x, y: F.t
+
+      proc aux(): group fset = {
+        var s;
+
+        x = $FDistr.dt;
+        y = $FDistr.dt;
+        s = A.solve(g ^ x, g ^ y);
+        return s;
+      }
+
+      proc main(): bool = {
+        var z, s;
+
+        s = aux();
+        z = $Duni.dU s;
+        return z = g ^ (x * y);
+      }
+    }.
+
+    lemma Reduction &m:
+      0 < n =>
+      1%r / n%r * Pr[SCDH(A).main() @ &m: res]
+      <= Pr[CDH.CDH(CDH_from_SCDH(A)).main() @ &m: res].
+    proof.
+      (* Move "0 < n" into the context *)
+      move=> n_pos.
+      (* We prove the inequality by transitivity:
+           1%r/n%r * Pr[SCDH(A).main() @ &m: res]
+           <= Pr[SCDH'.main() @ &m: res]
+           <= Pr[CDH.CDH(CDH_from_SCDH(A)).main() @ &m: res]. *)
+      (* "first last" allows us to first focus on the second inequality, which is easier. *)
+      apply (real_le_trans _ Pr[SCDH'.main() @ &m: res]); first last.
+        (* Pr[SCDH'.main() @ &m: res] <= Pr[CDH.CDH(CDH_from_SCDH(A)).main() @ &m: res] *)
+        (* This is in fact an equality, which we prove by program equivalence *)
+        byequiv (_: _ ==> ={res})=> //=.
+        by proc; inline *; auto; call (_: true); auto.
+      (* 1%r/n%r * Pr[SCDH(A).main() @ &m: res] <= Pr[SCDH'.main() @ &m: res] *)
+      (* We do this one using a combination of phoare (to deal with the final sampling of z)
+         and equiv (to show that SCDH'.aux and CDH.CDH are equivalent in context). *)
+      byphoare (_: (glob A) = (glob A){m} ==> _)=> //.
+      (* This line is due to a bug in proc *) pose d:= 1%r/n%r * Pr[SCDH(A).main() @ &m: res].
+      pose p:= Pr[SCDH(A).main() @ &m: res]. (* notation for ease of writing below *)
+      proc.
+      (* We split the probability computation into:
+           - the probability that s contains g^(x*y) and that |s| <= n is Pr[SCDH(A).main() @ &m: res], and
+           - when s contains g^(x*y), the probability of sampling that one element uniformly in s is bounded
+             by 1/n. *)
+      seq  1: (mem s (g ^ (SCDH'.x * SCDH'.y)) /\ card s <= n) p (1%r/n%r) _ 0%r => //. 
+        (* The first part is dealt with by equivalence with SCDH. *)
+        conseq (_: _: =p). (* strengthening >= into = for simplicity*)
+          call (_: (glob A) = (glob A){m}  ==> mem res (g^(SCDH'.x * SCDH'.y)) /\ card res <= n)=> //.
+            bypr; progress; rewrite /p.
+            byequiv (_: )=> //.
+            by proc *; inline *; wp; call (_: true); auto.
+      (* The second part is just arithmetic, but smt needs some help. *)
+      rnd (Pred.pred1 (g^(SCDH'.x * SCDH'.y))).
+      skip; progress.
+        rewrite Duni.mu_dU filter_pred1 H /= fcard1.
+        cut H1: 0 < card s{hr} by smt.
+        by rewrite -!Real.inv_def inv_le; smt.
+        smt.
+    qed.  
+  end section.
+
+end Set_CDH.
