theories/crypto/MAC.ec
@@ -1,0 +1,75 @@
+(* --------------------------------------------------------------------
+ * Copyright (c) - 2012--2015 - IMDEA Software Institute
+ * Copyright (c) - 2012--2015 - Inria
+ * 
+ * Distributed under the terms of the CeCILL-B-V1 license
+ * -------------------------------------------------------------------- *)
+
+require import FSet.
+
+type key.
+type message.
+type tag.
+
+module type Scheme = {
+  proc * init(): unit {}
+  proc keygen(): key
+  proc mac(k:key,m:message): tag
+  proc verify(k:key,m:message,t:tag): bool
+}.
+
+module type Oracles = {
+  proc mac(m:message): tag
+  proc verify(m:message,t:tag): bool
+}.
+
+module Wrap(S:Scheme) = {
+  var qs:message fset
+  var k:key
+
+  proc init(): unit = {
+    qs = fset0;
+    S.init();
+    k = S.keygen();
+  }
+
+  proc mac(m:message): tag = {
+    var r:tag;
+
+    qs = qs `|` fset1 m;
+    r = S.mac(k,m);
+    return r;
+  }
+
+  proc verify(m:message,t:tag): bool = {
+    var r:bool;
+
+    r = S.verify(k,m,t);
+    return r;
+  }
+
+  proc fresh(m:message): bool = {
+    return (!mem qs m);
+  }
+}.
+
+module type Adv_CMA(O:Oracles) = {
+  proc forge(): (message * tag)
+}.
+
+module CMA(S:Scheme,A:Adv_CMA) = {
+  module O = Wrap(S)
+  module A = A(O)
+
+  proc main(): bool = {
+    var m:message;
+    var t:tag;
+    var forged,fresh:bool;
+
+    O.init();
+    (m,t) = A.forge();
+    forged = O.verify(m,t);
+    fresh = O.fresh(m);
+    return forged /\ fresh;
+  }
+}.
