theories/crypto/PKS.ec
@@ -1,0 +1,154 @@
+(* --------------------------------------------------------------------
+ * Copyright (c) - 2012--2015 - IMDEA Software Institute
+ * Copyright (c) - 2012--2015 - Inria
+ * 
+ * Distributed under the terms of the CeCILL-B-V1 license
+ * -------------------------------------------------------------------- *)
+
+(* Definitions for Public-Key Signatures Schemes *)
+require import FSet.
+require import Pair.
+
+type pkey.
+type skey.
+type message.
+type signature.
+
+module type Scheme = {
+  proc * init(): unit {}
+  proc keygen(): (pkey * skey)
+  proc sign(sk:skey, m:message): signature
+  proc verify(pk:pkey, m:message, s:signature): bool
+}.
+
+module type AdvOracles = { proc sign(m:message): signature }.
+
+module type AdvCMA(O:AdvOracles) = {
+  proc forge(pk:pkey): (message * signature)
+}.
+
+theory EF_CMA.
+  module type Oracles = {
+    proc * init(): pkey {}
+    proc sign(m:message): signature
+    proc verify(m:message,s:signature): bool
+    proc fresh(m:message): bool
+    proc queries(): int
+  }.
+
+  (* A wrapper providing oracles for existential
+     unforgeability from a PKS scheme. *)
+  module Wrap(S:Scheme): Oracles = {
+    var qs: message fset
+    var pk: pkey
+    var sk: skey
+
+    proc init(): pkey = {
+      S.init();
+      qs = fset0;
+      (pk,sk) = S.keygen();
+      return pk;
+    }
+
+    proc sign(m:message): signature = {
+      var s:signature;
+      qs = qs `|` fset1 m;
+      s = S.sign(sk,m);
+      return s;
+    }
+
+    proc verify(m:message,s:signature): bool = {
+      var b:bool;
+      b = S.verify(pk,m,s);
+      return b;
+    }
+
+    proc fresh(m:message): bool = {
+      return !mem qs m;
+    }
+
+    proc queries(): int = {
+      return card qs;
+    }
+  }.
+
+  module EF_CMA(O:Oracles, A:AdvCMA) = {
+    module A = A(O)
+
+    proc main(): bool = {
+      var pk:pkey;
+      var m:message;
+      var s:signature;
+      var forged, fresh:bool;
+
+      pk = O.init();
+      (m,s) = A.forge(pk);
+      forged = O.verify(m,s);
+      fresh = O.fresh(m);
+      return forged /\ fresh;
+    }
+  }.
+end EF_CMA.
+
+theory NM_CMA.
+  module type Oracles = {
+    proc * init(): pkey {}
+    proc sign(m:message): signature
+    proc verify(m:message,s:signature): bool
+    proc fresh(m:message,s:signature): bool
+    proc queries(): int
+  }.
+
+  (* A wrapper providing oracles for
+     non-malleability from a PKS scheme. *)
+  module Wrap(S:Scheme): Oracles = {
+    var qs: (message * signature) fset
+    var pk: pkey
+    var sk: skey
+
+    proc init(): pkey = {
+      S.init();
+      qs = fset0;
+      (pk,sk) = S.keygen();
+      return pk;
+    }
+
+    proc sign(m:message): signature = {
+      var s:signature;
+      s = S.sign(sk,m);
+      qs = qs `|` fset1 (m,s);
+      return s;
+    }
+
+    proc verify(m:message,s:signature): bool = {
+      var b:bool;
+      b = S.verify(pk,m,s);
+      return b;
+    }
+
+    proc fresh(m:message,s:signature): bool = {
+      return !mem qs (m,s);
+    }
+
+    proc queries(): int = {
+      return card qs;
+    }
+  }.
+
+  module NM_CMA(O:Oracles, A:AdvCMA) = {
+    module A = A(O)
+
+    proc main(): bool = {
+      var pk:pkey;
+      var m:message;
+      var s:signature;
+      var forged, fresh:bool;
+
+      pk = O.init();
+      (m,s) = A.forge(pk);
+      forged = O.verify(m,s);
+      fresh = O.fresh(m,s);
+      return forged /\ fresh;
+    }
+  }.
+end NM_CMA.
