theories/crypto/ROM.ec
@@ -1,0 +1,1059 @@
+(* --------------------------------------------------------------------
+ * Copyright (c) - 2012--2015 - IMDEA Software Institute
+ * Copyright (c) - 2012--2015 - Inria
+ * 
+ * Distributed under the terms of the CeCILL-B-V1 license
+ * -------------------------------------------------------------------- *)
+
+require import FMap.
+require import Distr.
+
+theory Types.
+  type from.
+  type to.
+
+  (* Distribution to use on the target type; it can be parameterized by the input *)
+  op dsample: from -> to distr.
+
+  (* A signature for random oracles from "from" to "to". *)
+  module type Oracle =
+  {
+    proc init():unit
+    proc o (x:from):to
+  }.
+
+  module type ARO = {
+    proc o(x:from):to
+  }.
+
+  module type Dist (H:ARO) = {
+    proc distinguish(): bool
+  }.
+
+  module IND(H:Oracle,D:Dist) = {
+    module D = D(H)
+
+    proc main(): bool = {
+      var b:bool;
+
+      H.init();
+      b = D.distinguish();
+      return b;
+    }
+  }.
+end Types.
+
+theory Lazy.
+  require import FSet.
+
+  type from.
+  type to.
+
+  op dsample: from -> to distr.
+
+  clone export Types with
+    type from <- from,
+    type to <- to,
+    op dsample <- dsample.
+
+  module RO:Oracle = {
+    var m:(from, to) map
+
+    proc init():unit = {
+      m = FMap.empty;
+    }
+  
+    proc o(x:from):to = {
+      var y:to;
+      y = $dsample x;
+      if (!mem (dom m) x) m.[x] = y;
+      return oget (m.[x]);
+    }
+  }.
+
+  lemma RO_init_ll: islossless RO.init.
+  proof. by proc; wp. qed.
+
+  lemma RO_o_ll:
+    (forall x, mu (dsample x) predT = 1%r) =>
+    islossless RO.o.
+  proof. by intros=> dsampleL; proc; auto; smt. qed.
+
+  equiv RO_init_eq: RO.init ~ RO.init: true ==> ={glob RO}
+  by sim.
+
+  equiv RO_o_eq: RO.o ~ RO.o: ={glob RO, x} ==> ={glob RO, res}
+  by sim.
+
+  hoare dom_RO_o d x': RO.o: x = x' /\ dom RO.m = d ==> dom RO.m = d `|` fset1 x'.
+  proof. by proc; auto; smt. qed.
+end Lazy.
+
+theory Eager.
+  require import Finite.
+  require import FSet.
+
+  type from.
+  type to.
+
+  op dsample: from -> to distr.
+
+  clone export Types with
+    type from <- from,
+    type to <- to,
+    op dsample <- dsample.
+
+  module RO: Oracle = {
+    var m:(from,to) map
+
+    proc init(): unit = {
+      var y:to;
+      var work:from fset;
+      var f:from;
+
+      m = FMap.empty;
+      work = oflist (to_seq predT);
+      while (work <> fset0)
+      {
+        f = pick work;
+        y = $dsample f;
+        m.[f] = y;
+        work = work `\` fset1 f;
+      }
+    }
+
+    proc o(x:from): to = {
+      return oget m.[x];
+    }
+  }.
+
+  lemma RO_init_full:
+    is_finite predT<:from> =>
+    hoare [RO.init: true ==> forall x, FSet.mem (dom RO.m) x].
+  proof.
+    move=> fType; proc.
+    while (forall x, FSet.mem work x \/ mem (dom RO.m) x).
+      by auto; smt.
+    by auto; smt.
+  qed.
+
+  lemma RO_init_ll:
+    is_finite predT<:from> =>
+    (forall x, mu (dsample x) predT = 1%r) =>
+    islossless RO.init.
+  proof.
+    move=> fType dsampleL; proc.
+    while (true) (card work);
+    by auto; smt.
+  qed.
+
+  lemma RO_o_ll: islossless RO.o.
+  proof. by proc; wp. qed.
+
+  lemma RO_init_eq:
+    is_finite predT<:from> =>
+    equiv [RO.init ~ RO.init: true ==> ={glob RO}].
+  proof. by move=> fType; proc; while (={glob RO, work}); auto. qed.
+
+  equiv RO_o_eq: RO.o ~ RO.o: ={glob RO, x} ==> ={glob RO, res}
+  by sim.
+
+  lemma dom_RO_init x:
+    is_finite predT<:from> =>
+    hoare [RO.init: true ==> FSet.mem (dom RO.m) x].
+  proof. by move=> fType; proc; while (forall x, !FSet.mem work x => mem (dom RO.m) x); auto; smt. qed.
+end Eager.
+
+theory LazyEager.
+  require import Finite.
+  require import FSet.
+
+  type from.
+  type to.
+
+  op dsample: from -> to distr.
+
+  clone Types with
+    type from <- from,
+    type to <- to,
+    op dsample <- dsample.
+
+  clone export Lazy with
+    type from <- from,
+    type to <- to,
+    op dsample <- dsample.
+
+  clone export Eager with
+    type from <- from,
+    type to <- to,
+    op dsample <- dsample.
+
+  section.
+    declare module D:Dist {Lazy.RO,Eager.RO}.
+
+    local module IND_Lazy = {
+      module H:Oracle = {
+        var m:(from, to) map
+
+        proc init():unit = {
+          m = FMap.empty;
+        }
+
+        proc o(x:from):to = {
+          var y:to;
+          y = $dsample x;
+          if (!FSet.mem (dom m) x) m.[x] = y;
+          return oget (m.[x]);
+        }
+      }
+
+      proc resample(): unit = {
+        var work:from fset;
+        var f:from;
+        var y,y0:to;
+
+        work = oflist (to_seq predT);
+        while (work <> fset0)
+        {
+          f = pick work;
+          y = $dsample f;
+          if (!FSet.mem (dom H.m) f) H.m.[f] = y;
+          work = work `\` fset1 f;
+        }
+      }
+
+      module D = D(H)
+
+      proc main(): bool = {
+        var b:bool;
+
+        H.init();
+        b = D.distinguish();
+        resample();
+
+        return b;
+      }
+    }.
+
+    local lemma IND_Lazy:
+      is_finite predT<:from> =>
+      (forall x, mu (dsample x) predT = 1%r) =>
+      equiv [IND(Lazy.RO,D).main ~ IND_Lazy.main: ={glob D} ==> ={res}].
+    proof.
+      move=> fromF dsampleL; proc; seq 2 2: (={b}).
+        call (_: Lazy.RO.m{1} = IND_Lazy.H.m{2}); first by sim.
+        by call (_: ={glob D} ==> Lazy.RO.m{1} = IND_Lazy.H.m{2});
+          first by proc; wp.
+      inline IND_Lazy.resample;
+      while{2} (true) (card work{2});
+        first by auto; smt.
+      by auto; smt.
+    qed.
+
+    local module IND_Eager = {
+      module H = {
+        var m:(from,to) map
+
+        proc o(x:from): to = {
+          return oget (m.[x]);
+        }
+      }
+
+      proc resample(): unit = {
+        var work:from fset;
+        var f:from;
+        var y,y0:to;
+
+        work = oflist (to_seq predT);
+        while (work <> fset0)
+        {
+          f = pick work;
+          y = $dsample f;
+          if (!FSet.mem (dom H.m) f) H.m.[f] = y;
+          work = work `\` fset1 f;
+        }
+      }
+
+      module D = D(H)
+
+      proc main(): bool = {
+        var b:bool;
+
+        H.m = FMap.empty;
+        resample();
+        b = D.distinguish();
+
+        return b;
+      }
+    }.
+
+    local lemma eager_query:
+      is_finite predT<:from> =>
+      (forall x, mu (dsample x) predT = 1%r) =>
+      eager [IND_Eager.resample(); ,
+                 IND_Eager.H.o ~ IND_Lazy.H.o,
+             IND_Lazy.resample();:
+        ={x} /\ IND_Eager.H.m{1} = IND_Lazy.H.m{2} ==>
+        ={res} /\ IND_Eager.H.m{1} = IND_Lazy.H.m{2}].
+    proof.
+      move=> fromF dsampleL; eager proc.
+      inline IND_Eager.resample IND_Lazy.resample; swap{2} 4 -3.
+      seq 1 1: (={x,work} /\
+                IND_Eager.H.m{1} = IND_Lazy.H.m{2} /\
+                mem work{1} x{1});
+        first by auto; smt.
+      case (!mem (dom IND_Lazy.H.m{2}) x{2}); [rcondt{2} 2; first by auto |
+                                            rcondf{2} 2; first by auto].
+        transitivity{1} {y0 = $dsample x;
+                         while (work <> fset0) {
+                           f = pick work;
+                           y = $dsample f;
+                           if (!mem (dom IND_Eager.H.m) f)
+                             IND_Eager.H.m.[f] = if f = x then y0 else y;
+                           work = work `\` fset1 f;
+                         }
+                         result = oget IND_Eager.H.m.[x]; }
+                         (={x,work,IND_Eager.H.m} ==> ={result,IND_Eager.H.m})
+                         ((={x,work} /\
+                          IND_Eager.H.m{1} = IND_Lazy.H.m{2} /\
+                          mem work{1} x{1}) /\
+                          !mem (dom IND_Lazy.H.m{2}) x{2} ==>
+                          ={result} /\ IND_Eager.H.m{1} = IND_Lazy.H.m{2}) => //.
+          by move=> &1 &2 H; exists IND_Lazy.H.m{2}, x{2}, work{2}; generalize H.
+        transitivity{1} {while (work <> fset0) {
+                           f = pick work;
+                           y = $dsample f;
+                           if (!mem (dom IND_Eager.H.m) f)
+                             IND_Eager.H.m.[f] = y;
+                           work = work `\` fset1 f;
+                         }
+                         y0 = $dsample x;
+                         result = oget IND_Eager.H.m.[x]; }
+                         (={x,work,IND_Eager.H.m} ==> ={result,IND_Eager.H.m})
+                         (={x,work,IND_Eager.H.m} ==> ={result,IND_Eager.H.m})=> //.
+          by move=> &1 &2 H; exists IND_Eager.H.m{2}, x{2}, work{2}; generalize H.
+        by sim; rnd{2}; sim : (={x,IND_Eager.H.m}); smt.
+
+        wp; symmetry.
+        eager while (H:y0 = $dsample x; ~ y0 = $dsample x; : ={x} ==> ={y0})=> //; first by rnd.
+          swap{2} 5 -4; swap [2..3] -1; case ((x = pick work){1}).
+            by wp; rnd{2}; rnd; rnd{1}; wp; skip; smt.
+            by auto; smt.
+          by sim.
+
+        wp; while (={x, work} /\
+                   (!mem work x => mem (dom IND_Eager.H.m) x){1} /\
+                   IND_Lazy.H.m.[x]{2} = Some y0{1} /\
+                   if (mem (dom IND_Eager.H.m) x){1}
+                   then IND_Eager.H.m{1} = IND_Lazy.H.m{2}
+                   else eq_except IND_Eager.H.m{1} IND_Lazy.H.m{2} x{1}).
+          (* "expect 12 (move)" is used for catching changes in tactic behaviour early *)
+          auto; (progress; expect 12 move); last 2 first; first 11 smt.
+          case ((pick work = x){2})=> pick_x; last smt.
+          subst x{2}; generalize H7 H1; rewrite -neqF /eq_except=> -> /= eq_exc.
+          by apply map_ext=> x0; case (pick work{2} = x0); smt.
+        by auto; smt.
+
+      wp; while (={x,work} /\
+                 IND_Eager.H.m{1} = IND_Lazy.H.m{2} /\
+                 mem (dom IND_Lazy.H.m{2}) x{2} /\
+                 oget IND_Eager.H.m.[x]{1} = result{2}).
+         by auto; smt.
+      by auto; smt.
+    qed.
+
+    local lemma eager_aux:
+      is_finite predT<:from> =>
+      (forall x, mu (dsample x) predT = 1%r) =>
+      equiv [IND_Lazy.main ~ IND_Eager.main: ={glob D} ==> ={res}].
+    proof.
+      move=> fromF dsampleL; proc; inline IND_Lazy.H.init.
+      seq 1 1: (={glob D} /\ IND_Lazy.H.m{1} = IND_Eager.H.m{2}); first by wp.
+      symmetry.
+      eager (H: IND_Eager.resample(); ~ IND_Lazy.resample();:
+                  IND_Eager.H.m{1} = IND_Lazy.H.m{2} ==> IND_Eager.H.m{1} = IND_Lazy.H.m{2}): 
+            (={glob D} /\ IND_Eager.H.m{1} = IND_Lazy.H.m{2}) => //;
+        first by sim.
+      eager proc H (IND_Eager.H.m{1} = IND_Lazy.H.m{2})=> //;
+        first by apply eager_query.
+      by sim.
+    qed.
+
+    local lemma IND_Eager:
+      is_finite predT<:from> =>
+      (forall x, mu (dsample x) predT = 1%r) =>
+      equiv [IND_Eager.main ~ IND(Eager.RO,D).main: ={glob D} ==> ={res}].
+    proof.
+      move=> fromF dsampleL; proc.
+      call (_: (forall x, FSet.mem (dom IND_Eager.H.m{1}) x) /\ IND_Eager.H.m{1} = Eager.RO.m{2});
+        first by proc; skip; smt.
+      inline RO.init IND_Eager.resample.
+      while (={work} /\
+             (forall x, !FSet.mem (dom IND_Eager.H.m{1}) x <=>
+                        mem work{1} x) /\ IND_Eager.H.m{1} = Eager.RO.m{2}).
+        by auto; progress; smt.
+      by auto; smt.
+    qed.
+
+    lemma eagerRO:
+      is_finite predT<:from> =>
+      (forall x, mu (dsample x) predT = 1%r) =>
+      equiv [IND(Lazy.RO,D).main ~ IND(Eager.RO,D).main: ={glob D} ==> ={res}].
+    proof.
+      move=> fromF dsampleL; bypr (res{1}) (res{2})=> // &1 &2 a eq_D.
+      apply (eq_trans _ Pr[IND_Lazy.main() @ &1: a = res]);
+        first by byequiv (IND_Lazy _ _).
+      apply (eq_trans _ Pr[IND_Eager.main() @ &1: a = res]);
+        first by byequiv (eager_aux _ _).
+      by byequiv (IND_Eager _ _).
+    qed.
+  end section.
+end LazyEager.
+
+theory BoundedCall.
+  require import Int.
+
+  type from.
+  type to.
+
+  op dsample: from -> to distr.
+
+  op qH:int.
+
+  clone export Lazy with
+    type from  <- from,
+    type to    <- to,
+    op dsample <- dsample.
+
+  module Bound (O:Oracle) = {
+    var c:int
+
+    proc init(): unit = {
+      O.init();
+      c = 0;
+    }
+
+    proc o(x:from): to = {
+      var r = witness;
+
+      if (c < qH) {
+        r = O.o(x);
+        c = c + 1;
+      }
+      return r;
+    }
+  }.
+
+  lemma Bound_init_ll (O <: Oracle): islossless O.init => islossless Bound(O).init.
+  proof. by move=> O_init_ll; proc; wp; call O_init_ll. qed.
+
+  lemma Bound_o_ll (O <: Oracle): islossless O.o => islossless Bound(O).o.
+  proof. by move=> O_o_ll; proc; sp; if=> //; wp; call O_o_ll. qed.
+end BoundedCall.
+
+theory ListLog.
+  require import Int.
+  require import List.
+
+  type from.
+  type to.
+
+  op dsample: from -> to distr.
+
+  op qH:int.
+
+  clone export Lazy with
+    type from  <- from,
+    type to    <- to,
+    op dsample <- dsample.
+
+  module Log (O:Oracle) = {
+    var qs:from list
+
+    proc init(): unit = {
+      O.init();
+      qs = [];
+    }
+
+    proc o(x:from): to = {
+      var r:to;
+
+      qs = x::qs;
+      r = O.o(x);
+      return r;
+    }
+  }.
+
+  lemma Log_init_ll (O <: Oracle): islossless O.init => islossless Log(O).init.
+  proof. by move=> O_init_ll; proc; wp; call O_init_ll. qed.
+
+  lemma Log_o_ll (O <: Oracle): islossless O.o => islossless Log(O).o.
+  proof. by move=> O_oL; proc; call O_oL; wp. qed.
+
+  lemma Log_o_stable (O <: Oracle {Log}) q:
+    islossless O.o => phoare[Log(O).o: mem Log.qs q ==> mem Log.qs q] = 1%r.
+  proof. by move=> O_o_ll; proc; call O_o_ll; auto; progress; right. qed.
+
+  module Bound(O:Oracle) = {
+    module LO = Log(O)
+
+    proc init(): unit = {
+      Log(O).init();
+    }
+
+    proc o(x:from): to = {
+      var r = witness;
+
+      if (size Log.qs < qH) {
+        r = O.o(x);
+      }
+      return r;
+    }
+  }.
+end ListLog.
+
+theory SetLog.
+  require import Int.
+  require import FSet.
+
+  type from.
+  type to.
+
+  op dsample: from -> to distr.
+
+  op qH:int.
+
+  clone export Lazy with
+    type from  <- from,
+    type to    <- to,
+    op dsample <- dsample.
+
+  module Log(O:Oracle) = {
+    var qs:from fset
+
+    proc init(): unit = {
+      O.init();
+      qs = fset0;
+    }
+
+    proc o(x:from): to = {
+      var r;
+
+      r  = O.o(x);
+      qs = qs `|` fset1 x;
+      return r;
+    }
+  }.
+
+  lemma Log_init_ll (O <: Oracle): islossless O.init => islossless Log(O).init.
+  proof. by move=> O_init_ll; proc; wp; call O_init_ll. qed.
+
+  lemma Log_o_ll (O <: Oracle): islossless O.o => islossless Log(O).o.
+  proof. by move=> O_o_ll; proc; wp; call O_o_ll; wp. qed.
+
+  hoare Log_o_stable (O <: Oracle {Log}) x: Log(O).o: mem Log.qs x ==> mem Log.qs x.
+  proof. by proc; wp; call (_: true); skip; smt. qed.
+
+  hoare Log_o_Dom: Log(RO).o: Log.qs = dom RO.m ==> Log.qs = dom RO.m.
+  proof. proc; inline*; auto; smt. qed.
+
+  module Bound(O:Oracle) = {
+    module LO = Log(O)
+
+    proc init = Log(O).init
+
+    proc o(x:from): to = {
+      var r = witness;
+
+      if (card Log.qs < qH) {
+        r = LO.o(x);
+      }
+      return r;
+    }
+  }.
+
+  lemma Bound_init_ll (O <: Oracle): islossless O.init => islossless Bound(O).init.
+  proof. by move=> O_init_ll; proc; wp; call O_init_ll. qed.
+
+  lemma Bound_o_ll (O <: Oracle {Log}): islossless O.o => islossless Bound(O).o.
+  proof. by move=> O_o_ll; proc; sp; if=> //; wp; call (Log_o_ll O _). qed.
+
+  hoare Bound_o_stable (O <: Oracle {Log}) x: Bound(O).o: mem Log.qs x ==> mem Log.qs x.
+  proof. by proc; sp; if=> //; wp; call (Log_o_stable O x). qed.
+
+  equiv Log_Bound (O <: Oracle {Log}) (D <: Dist {O,Log}):
+    IND(Bound(O),D).main ~ IND(Log(Bound(O)),D).main: ={glob O, glob D} ==> ={res}.
+  proof.
+    proc.
+    call (_: ={glob O} /\ card Log.qs{1} <= card Log.qs{2} /\ (card Log.qs{1} < qH => ={glob Log})).
+      proc*; inline Log(Bound(O)).o Bound(O).o Bound(O).LO.o.
+      sp; if; first smt.
+        by wp; call (_: true); auto; smt.
+      auto; progress.
+        by apply/(Trans _ _ _ H)/subset_leq_fcard; smt.
+        smt.
+    by inline *; wp; call (_: true).
+  qed.
+end SetLog.
+
+theory ROM_BadCall.
+  (** A generic argument allowing us to replace a single random
+      oracle query with freshly sampled randomness. We then bound
+      the probability of distinguishing the two modules by the
+      probability of a third module that simply returns whether
+      the replaced query has been guessed by the adversary.       *)
+  (** We want to be able to:
+        1) express the result on Log(O);
+        2) and use it on Bound(O)...
+      HOW? *)
+  require import Int.
+  require import Real.
+  require import FSet.
+
+  type from.
+  type to.
+
+  op dsample: from -> to distr.
+  axiom dsampleL x: mu (dsample x) predT = 1%r.
+
+  op qH:int.
+
+  clone export SetLog with
+    type from  <- from,
+    type to    <- to,
+    op dsample <- dsample,
+    op qH      <- qH.
+
+  module type Dist(H:ARO) = {
+    proc a1(): from
+    proc a2(x:to): bool
+  }.
+
+  theory OnLog.
+    module G0(D:Dist, H:Oracle) = {
+      module D = D(Log(H))
+
+      proc main(): bool = {
+        var x, y, b;
+
+        Log(H).init();
+        x = D.a1();
+        y = H.o(x);
+        b = D.a2(y);
+        return b;
+      }
+    }.
+
+    module G1(D:Dist, H:Oracle) = {
+      module D = D(Log(H))
+
+      proc main(): bool = {
+        var x, y, b;
+
+        Log(H).init();
+        x = D.a1();
+        y = $dsample x;
+        b = D.a2(y);
+        return b;
+      }
+    }.
+
+    module G2(D:Dist, H:Oracle) = {
+      module D = D(Log(H))
+
+      proc main(): bool = {
+        var x, y, b;
+
+        Log(H).init();
+        x = D.a1();
+        y = $dsample x;
+        b = D.a2(y);
+        return mem Log.qs x;
+      }
+    }.
+
+    section.
+      declare module D : Dist {Log, RO}.
+      axiom Da1L (H <: Types.ARO {D}): islossless H.o => islossless D(H).a1.
+      axiom Da2L (H <: Types.ARO {D}): islossless H.o => islossless D(H).a2.
+
+      local module G1'(D:Dist, H:Oracle) = {
+        module D = D(Log(H))
+
+        var x:from
+
+        proc main(): bool = {
+          var y, b;
+
+          Log(H).init();
+          x = D.a1();
+          y = $dsample x;
+          b = D.a2(y);
+          return b;
+        }
+      }.
+
+      lemma ROM_BadCall &m:
+        Pr[G0(D,RO).main() @ &m: res] <= Pr[G1(D,RO).main() @ &m: res] + Pr[G2(D,RO).main() @ &m: res].
+      proof.
+        cut ->: Pr[G2(D,RO).main() @ &m: res] = Pr[G1'(D,RO).main() @ &m: mem Log.qs G1'.x].
+          byequiv (_: ={glob D} ==> res{1} = (mem Log.qs G1'.x){2})=> //.
+          proc.
+          call (_: ={glob Log, glob RO}); first by sim.
+          rnd; call (_: ={glob Log, glob RO}); first by sim.
+          by inline *; wp.
+        cut ->: Pr[G1(D,RO).main() @ &m: res] = Pr[G1'(D,RO).main() @ &m: res].
+          by byequiv (_: ={glob D} ==> ={res}); first by sim.
+        cut: Pr[G0(D,RO).main() @ &m: res] <= Pr[G1'(D,RO).main() @ &m: res \/ mem Log.qs G1'.x].
+          byequiv (_: ={glob D} ==> !mem Log.qs{2} G1'.x{2} => ={res})=> //; last smt.
+          proc.
+          call (_: mem Log.qs G1'.x,
+                   ={glob Log} /\
+                   Log.qs{2} = dom RO.m{2} /\
+                   eq_except RO.m{1} RO.m{2} G1'.x{2}).
+            by apply Da2L.
+            by proc; inline RO.o; auto; smt.
+            by progress; apply (Log_o_ll RO); apply (RO_o_ll _); smt.
+            progress; exists* G1'.x; elim* => x; conseq (Log_o_ll RO _) (Log_o_stable RO x)=> //.
+            by apply (RO_o_ll _); smt.
+          inline RO.o; auto.
+          call (_: ={glob Log, glob RO} /\ Log.qs{2} = dom RO.m{2}).
+            by proc; inline RO.o; auto; smt.
+          by inline Log(RO).init RO.init; auto; smt.
+        by rewrite Pr [mu_or]; smt.
+      qed.
+    end section.
+  end OnLog.
+
+  theory OnBound.
+    module G0(D:Dist, H:Oracle) = {
+      module D = D(Bound(H))
+
+      proc main(): bool = {
+        var x, y, b;
+
+        Bound(H).init();
+        x = D.a1();
+        y = H.o(x);
+        b = D.a2(y);
+        return b;
+      }
+    }.
+
+    module G1(D:Dist, H:Oracle) = {
+      module D = D(Bound(H))
+
+      proc main(): bool = {
+        var x, y, b;
+
+        Bound(H).init();
+        x = D.a1();
+        y = $dsample x;
+        b = D.a2(y);
+        return b;
+      }
+    }.
+
+    module G2(D:Dist, H:Oracle) = {
+      module D = D(Bound(H))
+
+      proc main(): bool = {
+        var x, y, b;
+
+        Bound(H).init();
+        x = D.a1();
+        y = $dsample x;
+        b = D.a2(y);
+        return mem Log.qs x;
+      }
+    }.
+
+    section.
+      declare module D : Dist {Log, RO}.
+      axiom Da1L (H <: Types.ARO {D}): islossless H.o => islossless D(H).a1.
+      axiom Da2L (H <: Types.ARO {D}): islossless H.o => islossless D(H).a2.
+
+      local module G1'(D:Dist, H:Oracle) = {
+        module D = D(Bound(H))
+
+        var x:from
+
+        proc main(): bool = {
+          var y, b;
+
+          Log(H).init();
+          x = D.a1();
+          y = $dsample x;
+          b = D.a2(y);
+          return b;
+        }
+      }.
+
+      lemma ROM_BadCall &m:
+        Pr[G0(D,RO).main() @ &m: res] <= Pr[G1(D,RO).main() @ &m: res] + Pr[G2(D,RO).main() @ &m: res].
+      proof.
+        cut ->: Pr[G2(D,RO).main() @ &m: res] = Pr[G1'(D,RO).main() @ &m: mem Log.qs G1'.x].
+          byequiv (_: ={glob D} ==> res{1} = (mem Log.qs G1'.x){2})=> //.
+          proc.
+          call (_: ={glob Log, glob RO}); first by sim.
+          rnd; call (_: ={glob Log, glob RO}); first by sim.
+          by inline *; wp.
+        cut ->: Pr[G1(D,RO).main() @ &m: res] = Pr[G1'(D,RO).main() @ &m: res].
+          by byequiv (_: ={glob D} ==> ={res}); first by sim.
+        cut: Pr[G0(D,RO).main() @ &m: res] <= Pr[G1'(D,RO).main() @ &m: res \/ mem Log.qs G1'.x].
+          byequiv (_: ={glob D} ==> !mem Log.qs{2} G1'.x{2} => ={res})=> //; last smt.
+          proc.
+          call (_: mem Log.qs G1'.x,
+                   ={glob Log} /\
+                   Log.qs{2} = dom RO.m{2} /\
+                   eq_except RO.m{1} RO.m{2} G1'.x{2}).
+            by apply Da2L.
+            by proc; inline Bound(RO).LO.o RO.o; sp; if=> //; auto; smt.
+            by progress; apply (Bound_o_ll RO); apply (RO_o_ll _); smt.
+            progress; exists* G1'.x; elim* => x; conseq (Bound_o_ll RO _) (Bound_o_stable RO x)=> //.
+            by apply (RO_o_ll _); smt.
+          inline RO.o; auto.
+          call (_: ={glob Log, glob RO} /\ Log.qs{2} = dom RO.m{2}).
+            by proc; inline Bound(RO).LO.o RO.o; sp; if=> //; auto; smt.
+          by inline Bound(RO).init Log(RO).init RO.init; auto; smt.
+        by rewrite Pr [mu_or]; smt.
+      qed.
+    end section.
+  end OnBound.    
+end ROM_BadCall.
+
+theory ROM_Bad.
+  (** This theory (and its final result FEL_ROM) abstracts away from the
+      Failure Event Lemma for Random Oracles, allowing it to be used at
+      a high-level of abstraction, without worrying about fel internals. *)
+  require import Int.
+  require import Real.
+  require import Sum. (* for the FEL tactic *)
+
+  type from.
+  type to.
+
+  op dsample: from -> to distr.
+  axiom dsampleL x: mu (dsample x) predT = 1%r.
+
+  op qH:int.
+  axiom qH_pos: 0 < qH.
+
+  clone export BoundedCall with
+    type from  <- from,
+    type to    <- to,
+    op dsample <- dsample,
+    op qH      <- qH.
+
+  module type Dist(H:Oracle) = {
+    proc distinguish(): bool {H.o}
+  }.
+
+  module Experiment(H:Oracle,D:Dist) = {
+    module D = D(Bound(H))
+
+    proc main(): bool = {
+      var b;
+
+      Bound(H).init();
+      b = D.distinguish();
+      return b;
+    }
+  }.
+
+  section.
+    (** Note that the proof does not depend at all on the fact that O1 and O2
+        are random oracles. This argument could (and should) be generalized to
+        any two oracles whose probability of behaving differently on a single
+        query is bounded. *)
+    declare module O1 : Oracle {Bound}.
+    axiom O1_o_ll: islossless O1.o.
+
+    declare module O2 : Oracle {O1,Bound}.
+    axiom O2_o_ll: islossless O2.o.
+
+    declare module D : Dist {O1,O2,Bound}.
+    axiom D_distinguish_ll (O <: Oracle {D}): islossless O.o => islossless D(O).distinguish.
+
+    lemma FEL_ROM (bad: (glob O2) -> bool)
+                  (Phi: (glob O1) -> (glob O2) -> bool) eps &m:
+      0%r <= eps => (* should be derivable from phoare but isn't *)
+      hoare [O2.init: true ==> !bad (glob O2)] =>
+      equiv [O1.init ~ O2.init: true ==> Phi (glob O1){1} (glob O2){2}] =>
+      hoare [O2.o: bad (glob O2) ==> bad (glob O2)] =>
+      phoare [O2.o: !bad (glob O2) ==> bad (glob O2)] <= eps =>
+      equiv [O1.o ~ O2.o: !bad (glob O2){2} /\ ={x} /\ Phi (glob O1){1} (glob O2){2} ==>
+                          !bad (glob O2){2} => ={res} /\ Phi (glob O1){1} (glob O2){2}] =>
+      Pr[Experiment(O1,D).main() @ &m: res] <= Pr[Experiment(O2,D).main() @ &m: res] + qH%r * eps.
+    proof.
+      move=> eps_pos badinit eq_init bad_preserved bad1 eq_upto.
+      apply (Trans _ (Pr[Experiment(O2,D).main() @ &m: res] + Pr[Experiment(O2,D).main() @ &m: bad (glob O2)])).
+        cut: Pr[Experiment(O1,D).main() @ &m: res] <= Pr[Experiment(O2,D).main() @ &m: res \/ bad (glob O2)].
+          byequiv (_: ={glob D} ==> !bad (glob O2){2} => ={res})=> //; last smt.
+          proc.
+          call (_: bad (glob O2),
+                   ={glob Bound} /\
+                   Phi (glob O1){1} (glob O2){2}).
+            by apply D_distinguish_ll.
+            by proc; sp; if=> //; wp; call eq_upto.
+            by progress; proc; sp; if=> //; wp; call O1_o_ll.
+            by progress; proc; sp; if=> //; wp;
+               call (_: bad (glob O2) ==> bad (glob O2));
+                 first by conseq O2_o_ll bad_preserved.
+          call (_: true ==> ={glob Bound} /\ Phi (glob O1){1} (glob O2){2} /\ !bad (glob O2){2}).
+            proc; inline Bound(O1).init Bound(O2).init; wp.
+            by call (_: true ==> Phi (glob O1){1} (glob O2){2} /\ !bad (glob O2){2});
+                 first conseq eq_init _ badinit=> //.
+          by skip; smt.
+        by rewrite Pr [mu_or]; smt.
+      cut: Pr[Experiment(O2,D).main() @ &m: bad (glob O2)] <= qH%r * eps.
+        cut ->: Pr[Experiment(O2,D).main() @ &m: bad (glob O2)]
+                = Pr[Experiment(O2,D).main() @ &m: bad (glob O2) /\ Bound.c <= qH].
+          byequiv (_: ={glob D, glob O2} ==> bad (glob O2){1} <=> bad (glob O2){2} /\ Bound.c{2} <= qH)=> //.
+          proc.
+          call (_: ={glob O2, glob Bound} /\ Bound.c{2} <= qH)=> //.
+            by proc; sp; if=> //; wp; call (_: true); skip; smt.
+          call (_: ={glob O2} ==> ={glob O2, glob Bound} /\ Bound.c{2} <= qH).
+            by proc*; inline Bound(O2).init; wp; call (_: true); skip; smt.
+          done.
+        fel 1 Bound.c (fun x, eps) qH (bad (glob O2)) [Bound(O2).o: (Bound.c < qH)]=> //.
+          by rewrite Sum.int_sum_const //= Sum.intval_card_0 smt.
+          by call (_: true ==> !bad (glob O2) /\ Bound.c = 0);
+            first proc; wp; call badinit.
+          proc; sp; if=> //; last by hoare.
+          by wp; call (_: !bad (glob O2) ==> bad (glob O2)).
+          by progress; proc; sp; if=> //; wp; call (_: true); skip; smt.
+          by progress; proc; rcondf 2; auto; smt.
+      smt.
+    qed.
+  end section.
+end ROM_Bad.
+
+(*
+theory Wrappers.
+  clone import Types.
+  clone Lazy with
+    type from = from,
+    type to = to,
+    op dsample = dsample.
+
+  module type WRO = {
+    proc init(qO:int): unit {}
+    proc o(x:from): to
+  }.
+
+  module IND_b(H:WRO,D:Dist) = {
+    module D = D(H)
+
+    proc main(qO:int): bool = {
+      var b:bool;
+      H.init(qO);
+      b = D.distinguish();
+      return b;
+    }
+  }.
+
+  (** Budget-cutting wrapper *)
+  require import Int.
+  module Count(H:Oracle) = {
+    var qO:int
+    var qs:int
+
+    proc init(qO:int): unit = {
+      H.init();
+      Count.qO = qO;
+      qs = 0;
+    }
+
+    proc o(x:from): to = {
+      var r:to;
+      if (qs < qO)
+      {
+        qs = qs + 1;
+        r = H.o(x);
+      }
+      return r;
+    }
+  }.
+
+  import FSet.
+  import ISet.Finite.
+  lemma bound qO' (D <: Dist {Lazy.RO,Count}):
+    0 < qO' =>
+    (forall x, mu (dsample x) cpTrue = 1%r) =>
+    (forall (H <: ARO {D}), islossless H.o => islossless D(H).distinguish) =>
+    equiv [ IND(Lazy.RO,D).main ~ IND_b(Count(Lazy.RO),D).main:
+              qO{2} = qO' ==>
+              (Count.qs{2} < qO' =>
+                 ={res} /\
+                 size Lazy.RO.m{1} <= Count.qs{2}) ].
+  proof strict.
+  intros=> lt0_qO dsampleL DL; proc.
+  call (_: Count.qO <= Count.qs,
+           ={glob Lazy.RO} /\
+           Count.qO{2} = qO' /\
+           size Lazy.RO.m{1} <= Count.qs{2}).
+    (* H *)
+    proc; rcondt{2} 1; first intros=> &m; skip; progress=> //; smt.
+      inline Lazy.RO.o; wp; rnd; wp; skip; progress=> //; last smt.
+        by rewrite /size dom_set card_add_nin -/(in_dom _ _); last smt.
+    by intros=> _ _; apply Lazy.lossless_o.
+    by intros=> _; proc; if=> //; inline Lazy.RO.o; wp; rnd; wp; skip; smt.
+  inline Count(Lazy.RO).init; wp; call (_: true ==> ={glob Lazy.RO} /\ dom Lazy.RO.m{1} = FSet.empty)=> //;
+    first by proc; wp; skip; progress=> //; smt.
+  wp; skip; cut H1: ISet.empty<:from> == FSet.empty by smt; progress=> //.
+    by rewrite /size H card_empty.
+    by cut [eq_res _]:= H2 _; first smt.
+    by cut [_ [_ [fdom _]]]:= H2 _; first smt.
+  qed.
+
+(*
+  (** Query-tracking wrapper *)
+  require import Int.
+  module Index(H:Oracle) = {
+    var qs:(int,from) map
+    var qc:int
+
+    fun init(): unit = {
+      H.init();
+      qs = FMap.Core.empty;
+      qc = 0;
+    }
+
+    fun o(x:from): to = {
+      var r:to;
+      if (!in_rng x qs)
+      {
+        qs.[qc] = x;
+        qc = qc + 1;
+      }
+      r = H.o(x);
+      return r;
+    }
+  }.
+*)
+  (** Query-numbering wrapper *)
+  module Number(H:Oracle) = {
+    var qs:(from,int) map
+    var qc:int
+
+    proc init(): unit = {
+      H.init();
+      qs = FMap.empty;
+      qc = 0;
+    }
+
+    proc o(x:from): to = {
+      var r:to;
+      if (!in_dom x qs)
+      {
+        qs.[x] = qc;
+        qc = qc + 1;
+      }
+      r = H.o(x);
+      return r;
+    }
+  }.
+end Wrappers.
+*)
+
