theories/crypto/SecureChannels.ec
@@ -1,0 +1,119 @@
+(* --------------------------------------------------------------------
+ * Copyright (c) - 2012--2015 - IMDEA Software Institute
+ * Copyright (c) - 2012--2015 - Inria
+ * 
+ * Distributed under the terms of the CeCILL-B-V1 license
+ * -------------------------------------------------------------------- *)
+
+require import Bool.
+require import Int.
+require import Option.
+require import FSet.
+
+type key.
+type message.
+type container.
+
+module type Scheme = {
+  proc init(): unit
+  proc kg(): key
+  proc send(k:key,m:message): container
+  proc recv(k:key,c:container): message option
+}.
+
+theory MultiUser.
+  require import Array.
+
+  const users:int.
+  axiom users_pos: 0 < users.
+
+  module type Oracles = {
+    proc send(i:int,m0:message,m1:message): container option
+    proc recv(i:int,c:container): message option
+  }.
+
+  module Wrap(S:Scheme) = {
+    var qs:message fset
+    var ks:key array
+    var b:bool
+    var auth:bool
+
+    proc initKeys(): unit = {
+      var i:int;
+
+      i = 0;
+      while (i < users)
+      {
+        ks.[i] = S.kg();
+        i = i + 1;
+      }
+    }
+
+    proc init(): unit = {
+      qs = fset0;
+      auth = false;
+      S.init();
+      b = ${0,1};
+      initKeys();
+    }
+
+    proc send(i:int,m0:message,m1:message): container option = {
+      var r:container option;
+      var c:container;
+
+      if (0 <= i < users)
+      {
+        qs = qs `|` (fset1 m0) `|` (fset1 m1);
+        c = S.send(ks.[i],b ? m1 : m0);
+        r = Some c;
+      }
+      else
+        r = None;
+
+      return r;      
+    }
+
+    proc recv(i:int,c:container): message option = {
+      var r:message option;
+
+      if (0 <= i < users)
+      {
+        r = S.recv(ks.[i],c);
+        if (r <> None /\ !mem qs (oget r))
+          auth = true;
+      }
+      else
+        r = None;
+      return r;
+    }
+
+    proc guess(b':bool): bool = {
+      return b' = b;
+    }
+
+    proc auth(): bool = {
+      return auth;
+    }
+  }.
+
+  module type Adv_LOR(O:Oracles) = {
+    proc guess(): bool
+  }.
+
+  module LOR(S:Scheme,A:Adv_LOR) = {
+    module O = Wrap(S)
+    module A = A(O)
+
+    proc main(): bool = {
+      var b',sec,auth:bool;
+
+      O.init();
+      b' = A.guess();
+      sec = O.guess(b');
+      auth = O.auth();
+      return sec \/ auth;
+    }
+  }.
+end MultiUser.
+
+(* Reduce multi-user to single-user *)
