theories/crypto/SymmetricEncryption.ec
@@ -1,0 +1,128 @@
+(* --------------------------------------------------------------------
+ * Copyright (c) - 2012--2015 - IMDEA Software Institute
+ * Copyright (c) - 2012--2015 - Inria
+ * 
+ * Distributed under the terms of the CeCILL-B-V1 license
+ * -------------------------------------------------------------------- *)
+
+require import Option.
+require import Bool.
+require import List.
+
+type key.
+type plaintext.
+type ciphertext.
+
+module type Scheme = {
+  proc * init(): unit {}
+  proc kg(): key
+  proc enc(k:key,p:plaintext): ciphertext
+  proc dec(k:key,c:ciphertext): plaintext option
+}.
+
+module type CPA_Oracles = {
+  proc enc(p:plaintext): ciphertext
+}.
+
+module type CCA_Oracles = {
+  proc enc(p:plaintext): ciphertext
+  proc dec(c:ciphertext): plaintext option
+}.
+
+module type Adv_INDCPA (O:CPA_Oracles) = {
+  proc choose(): plaintext * plaintext
+  proc guess(c:ciphertext): bool
+}.
+
+module type Adv_INDCCA (O:CCA_Oracles) = {
+  proc choose(): plaintext * plaintext
+  proc guess(c:ciphertext): bool
+}.
+
+module Wrap (S:Scheme) = {
+  var k:key
+  var qs:ciphertext list
+
+  proc init(): unit = {
+    S.init();
+    k = S.kg();
+    qs = [];
+  }
+
+  proc enc(p:plaintext): ciphertext = {
+    var r:ciphertext;
+
+    r = S.enc(k,p);
+    return r;
+  }
+
+  proc dec(c:ciphertext): plaintext option = {
+    var r:plaintext option;
+
+    qs = c::qs;
+    r = S.dec(k,c);
+    return r;
+  }
+
+  proc queried_challenge(c:ciphertext): bool = {
+    return mem qs c;
+  }
+}.
+
+module INDCPA (S:Scheme, A:Adv_INDCPA) = {
+  module O = Wrap(S)
+  module A = A(O)
+
+  proc main(): bool = {
+    var b, b':bool;
+    var p, p0, p1:plaintext;
+    var c:ciphertext;
+
+    O.init();
+    (p0,p1) = A.choose();
+    b = ${0,1};
+    p = if b then p1 else p0;
+    c = O.enc(p);
+    b' = A.guess(c);
+    return (b = b');
+  }
+}.
+
+module INDCCA (S:Scheme, A:Adv_INDCCA) = {
+  module O = Wrap(S)
+  module A = A(O)
+
+  proc main(): bool = {
+    var b, b', qc:bool;
+    var p, p0, p1:plaintext;
+    var c:ciphertext;
+
+    O.init();
+    (p0,p1) = A.choose();
+    b = ${0,1};
+    p = if b then p1 else p0;
+    c = O.enc(p);
+    b' = A.guess(c);
+    qc = O.queried_challenge(c);
+    return (b = b' /\ !qc);
+  }
+}.
+
+module ToCCA (A:Adv_INDCPA, O:CCA_Oracles) = A(O).
+
+lemma CCA_implies_CPA (S <: Scheme {INDCPA}) (A <: Adv_INDCPA {S, INDCPA}) &m:
+  Pr[INDCPA(S,A).main() @ &m: res] = Pr[INDCCA(S,ToCCA(A)).main() @ &m: res].
+proof strict.
+byequiv (_: ={glob A} ==> ={res})=> //; proc.
+call{2} (_: Wrap.qs = [] ==> !res); first by proc; skip; smt.
+conseq [-frame] (_: _ ==> Wrap.qs{2} = [] /\ (b = b'){1} = (b = b'){2}); first smt.
+call (_: ={glob Wrap, glob S} /\ Wrap.qs{2} = []);
+  first by proc; call (_: true).
+call (_: ={glob Wrap, glob S});
+  first by call (_: true).
+wp; rnd.
+call (_: ={glob Wrap, glob S} /\ Wrap.qs{2} = []);
+  first by proc; call (_: true).
+by call (_: true ==> ={glob Wrap, glob S} /\ Wrap.qs{2} = []);
+     first by proc; wp; sim.
+qed.
