theories/newth/RealExtra.ec
@@ -1,0 +1,30 @@
+(* --------------------------------------------------------------------
+ * Copyright (c) - 2012--2015 - IMDEA Software Institute
+ * Copyright (c) - 2012--2015 - Inria
+ * 
+ * Distributed under the terms of the CeCILL-B-V1 license
+ * -------------------------------------------------------------------- *)
+
+(* -------------------------------------------------------------------- *)
+require export Real.
+
+pragma +implicits.
+
+(* -------------------------------------------------------------------- *)
+op lub (E : real -> bool) : real.
+
+pred nonempty (E : real -> bool) =
+  exists x, E x.
+
+pred ub (E : real -> bool) (z : real) =
+  forall y, E y => y <= z.
+
+pred has_ub  (E : real -> bool) = nonempty (ub E).
+pred has_lub (E : real -> bool) = nonempty E /\ has_ub E.
+
+axiom lub_upper_bound (E : real -> bool): has_lub E => 
+  forall x, E x => x <= lub E.
+
+axiom lub_adherent (E : real -> bool): has_lub E =>
+  forall eps, 0%r < eps =>
+    exists e, E e /\ (lub E - eps) < e.
