theories/newth/RealSeq.ec
@@ -1,0 +1,96 @@
+(* --------------------------------------------------------------------
+ * Copyright (c) - 2012--2015 - IMDEA Software Institute
+ * Copyright (c) - 2012--2015 - Inria
+ * 
+ * Distributed under the terms of the CeCILL-B-V1 license
+ * -------------------------------------------------------------------- *)
+
+(* -------------------------------------------------------------------- *)
+require import Bool Option Fun Distr Int IntExtra Real RealExtra.
+require import StdRing StdOrder StdBigop List Array.
+(*---*) import IterOp BRA RField RealOrder.
+
+pragma +implicits.
+
+(* -------------------------------------------------------------------- *)
+op convergeto (s : int -> real) (x : real) =
+  forall epsilon, 0%r < epsilon => exists N,
+    forall n, (N <= n)%Int => `|s n - x| < epsilon.
+
+op converge (s : int -> real) =
+  exists l, convergeto s l.
+
+op bounded_by (s : int -> real) (M : real) =
+  exists N, forall n, (N <= n)%Int => `|s n| <= M.
+
+op bounded (s : int -> real) =
+  exists M, bounded_by s M.
+
+op monotone (s : int -> real) =
+  forall n, 0 <= n => s n <= s (n+1).
+
+(* -------------------------------------------------------------------- *)
+lemma monotoneP (s : int -> real):
+  monotone s <=> (forall m n, 0 <= m <= n => s m <= s n).
+proof. admit. qed.
+
+lemma uniq_cnv s x y: convergeto s x => convergeto s y => x = y.
+proof.
+move=> lim_sx lim_sy; case: (x = y)=> // ne_xy.
+pose e := `|x - y| / 2%r; have gt0e: 0%r < e.
+  by rewrite /e divr_gt0 ?(normr_gt0, subr_eq0).
+case: (lim_sx _ gt0e) => {lim_sx} Nx lim_sx.
+case: (lim_sy _ gt0e) => {lim_sy} Ny lim_sy.
+case: (max_is_ub Nx Ny); (pose N := max _ _).
+move=> /lim_sx {lim_sx} lim_sx /lim_sy {lim_sy} lim_sy.
+have := ltr_add _ _ _ _ lim_sx lim_sy; rewrite ltrNge.
+by rewrite /e double_half @(distrC (s N)) ler_dist_add.
+qed.
+
+lemma eq_cnv s1 s2 l:
+     (exists N, forall n, (N <= n)%Int => s1 n = s2 n)
+  => convergeto s1 l => convergeto s2 l.
+proof.
+case=> N eq_s lim_s1 e gt0_e; case: (lim_s1 _ gt0_e).
+move=> Ns lim_s1N; exists (max N Ns)=> n /geq_max [leN leNs].
+by rewrite -eq_s // lim_s1N.
+qed.
+
+lemma le_cnv s1 s2 l1 l2:
+     (exists N, forall n, (N <= n)%Int => (s1 n <= s2 n)%Real)
+  => convergeto s1 l1 => convergeto s2 l2 => l1 <= l2.
+proof. admit. qed.
+
+lemma cnvC c: convergeto (fun x => c) c.
+proof. admit. qed.
+
+lemma cnvD s1 s2 l1 l2: convergeto s1 l1 => convergeto s2 l2 =>
+  convergeto (fun x => s1 x + s2 x) (l1 + l2).
+proof. admit. qed.
+
+lemma cnvB s l: convergeto s l => convergeto (fun x => -(s x)) (-l).
+proof. admit. qed.
+
+lemma cnvM s1 s2 l1 l2: convergeto s1 l1 => convergeto s2 l2 =>
+  convergeto (fun x => s1 x * s2 x) (l1 * l2).
+proof. admit. qed.
+
+lemma cnvZ c s l: convergeto s l => convergeto (fun x => c * s x) l.
+proof. admit. qed.
+
+lemma cnvM_bounded s1 s2: convergeto s1 0%r => bounded s2 => 
+  convergeto (fun x => s1 x * s2 x) 0%r.
+proof. admit. qed.
+  
+(* -------------------------------------------------------------------- *)
+op lim (s : int -> real) =
+  choiceb (fun l => convergeto s l) 0%r.
+
+(* -------------------------------------------------------------------- *)
+lemma limP (s : int -> real):
+  converge s <=> convergeto s (lim s).
+proof. by split=> [/choicebP /(_ 0%r)|lims]; last exists (lim s). qed.
+
+lemma lim_Ncnv (s : int -> real):
+  ! converge s => lim s = 0%r.
+proof. by move=> h; apply/choiceb_dfl/for_ex. qed.
