theories/newth/RealSeries.ec
@@ -1,0 +1,20 @@
+(* --------------------------------------------------------------------
+ * Copyright (c) - 2012--2015 - IMDEA Software Institute
+ * Copyright (c) - 2012--2015 - Inria
+ * 
+ * Distributed under the terms of the CeCILL-B-V1 license
+ * -------------------------------------------------------------------- *)
+
+(* -------------------------------------------------------------------- *)
+require import Bool Option Fun Distr Int IntExtra Real RealExtra.
+require import StdRing StdOrder StdBigop List RealSeq.
+(*---*) import IterOp BRA.
+
+pragma +implicits.
+
+(* -------------------------------------------------------------------- *)
+op partial (s : int -> real) (n : int) : real =
+  BRA.bigi predT s 0 n.
+
+pred convergeto (s : int -> real) (x : real) =
+  RealSeq.convergeto (partial s) x.
