theories/newth/distributions/FSet/Drestrict.ec
@@ -1,0 +1,24 @@
+(* --------------------------------------------------------------------
+ * Copyright (c) - 2012-2015 - IMDEA Software Institute and INRIA
+ * Distributed under the terms of the CeCILL-B licence.
+ * -------------------------------------------------------------------- *)
+
+(* -------------------------------------------------------------------- *)
+require import Int Real Distr FSet.
+
+pragma +implicits.
+
+(* -------------------------------------------------------------------- *)
+op drestr: 'a distr -> 'a fset -> 'a distr.
+
+axiom supp_def (x:'a) d X:
+  in_supp x (drestr d X) <=> in_supp x d /\ !mem X x.
+
+axiom mu_x_def_notin (x:'a) d (X:'a fset):
+  in_supp x d => !mem X x => mu_x (drestr d X) x = mu_x d x.
+
+lemma nosmt mu_x_def_in (x:'a) d (X:'a fset):
+  in_supp x d => mem X x => mu_x (drestr d X) x = 0%r by [].
+
+axiom weight_def (d:'a distr) X:
+  weight (drestr d X) = weight d - mu d (mem X).
